src/SDK/Materials.dfy
@@ -2,15 +2,14 @@ include "../StandardLibrary/StandardLibrary.dfy"
 include "../StandardLibrary/UInt.dfy"
 include "./AlgorithmSuite.dfy"
 include "../Util/UTF8.dfy"
+include "EncryptionContext.dfy"
 
 module {:extern "Materials"} Materials {
   import opened StandardLibrary
   import opened UInt = StandardLibrary.UInt
   import UTF8
   import AlgorithmSuite
-
-
-  type EncryptionContext = map<UTF8.ValidUTF8Bytes, UTF8.ValidUTF8Bytes>
+  import EncryptionContext
 
   // UTF-8 encoded "aws-crypto-public-key"
   const EC_PUBLIC_KEY_FIELD: UTF8.ValidUTF8Bytes :=
@@ -72,7 +71,7 @@ module {:extern "Materials"} Materials {
     && (plaintextDataKey.None? ==> |keyringTrace| == 0)
   }
 
-  datatype EncryptionMaterials = EncryptionMaterials(encryptionContext: EncryptionContext,
+  datatype EncryptionMaterials = EncryptionMaterials(encryptionContext: EncryptionContext.T,
                                                      algorithmSuiteID: AlgorithmSuite.ID,
                                                      plaintextDataKey: Option<seq<uint8>>,
                                                      encryptedDataKeys: seq<ValidEncryptedDataKey>,
@@ -85,13 +84,15 @@ module {:extern "Materials"} Materials {
       && GenerateTraceEntriesConsistent(plaintextDataKey, keyringTrace)
       && |Filter(keyringTrace, IsEncryptTraceEntry)| == |encryptedDataKeys|
       // TODO: Strongly tie each trace entry to it's corresponding EDK (https://github.com/awslabs/aws-encryption-sdk-dafny/issues/100)
+//      && |encryptedDataKeys| > 0 // KRML new
+//      && Context.ValidAAD(encryptionContext) // KRML new
     }
 
     static function method ValidWitness(): EncryptionMaterials {
       EncryptionMaterials(map[], AlgorithmSuite.AES_256_GCM_IV12_TAG16_HKDF_SHA384_ECDSA_P384, None, [], [], Some(seq(32, i => 0)))
     }
 
-    static function method WithoutDataKeys(encryptionContext: EncryptionContext,
+    static function method WithoutDataKeys(encryptionContext: EncryptionContext.T,
                                            algorithmSuiteID: AlgorithmSuite.ID,
                                            signingKey: Option<seq<uint8>>): ValidEncryptionMaterials 
       requires algorithmSuiteID.SignatureType().Some? ==> signingKey.Some?
@@ -132,7 +133,7 @@ module {:extern "Materials"} Materials {
   type ValidEncryptionMaterials = i: EncryptionMaterials | i.Valid() witness EncryptionMaterials.ValidWitness()
 
   datatype DecryptionMaterials = DecryptionMaterials(algorithmSuiteID: AlgorithmSuite.ID,
-                                                     encryptionContext: EncryptionContext,
+                                                     encryptionContext: EncryptionContext.T,
                                                      plaintextDataKey: Option<seq<uint8>>,
                                                      verificationKey: Option<seq<uint8>>,
                                                      keyringTrace: seq<KeyringTraceEntry>)
@@ -149,7 +150,7 @@ module {:extern "Materials"} Materials {
                           [KeyringTraceEntry([], [], {DECRYPTED_DATA_KEY})])
     }
 
-    static function method WithoutPlaintextDataKey(encryptionContext: EncryptionContext,
+    static function method WithoutPlaintextDataKey(encryptionContext: EncryptionContext.T,
                                                    algorithmSuiteID: AlgorithmSuite.ID,
                                                    verificationKey: Option<seq<uint8>>): ValidDecryptionMaterials 
       requires algorithmSuiteID.SignatureType().Some? ==> verificationKey.Some?
@@ -179,13 +180,13 @@ module {:extern "Materials"} Materials {
 
   type ValidDecryptionMaterials = i: DecryptionMaterials | i.Valid() witness DecryptionMaterials.ValidWitness()
 
-  datatype EncryptionMaterialsRequest = EncryptionMaterialsRequest(encryptionContext: EncryptionContext,
+  datatype EncryptionMaterialsRequest = EncryptionMaterialsRequest(encryptionContext: EncryptionContext.T,
                                                                    algorithmSuiteID: Option<AlgorithmSuite.ID>,
                                                                    plaintextLength: Option<nat>)
 
   datatype DecryptionMaterialsRequest = DecryptionMaterialsRequest(algorithmSuiteID: AlgorithmSuite.ID,
                                                                    encryptedDataKeys: seq<ValidEncryptedDataKey>,
-                                                                   encryptionContext: EncryptionContext)
+                                                                   encryptionContext: EncryptionContext.T)
   {
     predicate Valid() {
       |encryptedDataKeys| > 0
