src/SDK/EncryptionContext.dfy
@@ -1,0 +1,341 @@
+include "../StandardLibrary/StandardLibrary.dfy"
+include "../StandardLibrary/UInt.dfy"
+include "../Util/UTF8.dfy"
+include "../Util/Sets.dfy"
+
+module {:extern "EncryptionContext"} EncryptionContext {
+  import opened StandardLibrary
+  import opened UInt = StandardLibrary.UInt
+  import UTF8
+  import Sets
+
+  /*
+   * The main type of encryption context
+   */
+
+  type T = map<UTF8.ValidUTF8Bytes, UTF8.ValidUTF8Bytes>
+
+  predicate {:opaque} ValidAAD(encryptionContext: T) {
+    && KVPairsLength(encryptionContext) < UINT16_LIMIT
+    && ValidKVPairs(encryptionContext)
+  }
+
+  /*
+   * Validity of key-value pairs in the encryption context
+   */
+
+  predicate method ValidKVPairs(encryptionContext: T) {
+    && |encryptionContext| < UINT16_LIMIT
+    && (forall key :: key in encryptionContext.Keys ==> ValidKVPair((key, encryptionContext[key])))
+  }
+
+  predicate method ValidKVPair(kvPair: (UTF8.ValidUTF8Bytes, UTF8.ValidUTF8Bytes)) {
+    && |kvPair.0| < UINT16_LIMIT
+    && |kvPair.1| < UINT16_LIMIT
+    && UTF8.ValidUTF8Seq(kvPair.0)
+    && UTF8.ValidUTF8Seq(kvPair.1)
+  }
+
+  /*
+   * Length properties
+   */
+
+  function KVPairsLength(encryptionContext: T): nat
+  {
+    if |encryptionContext| == 0 then 0 else
+      // Defining and reasoning about order at this level is simplified by using a sequence of
+      // key value pairs instead of a map.
+      var keys: seq<UTF8.ValidUTF8Bytes> := SetToOrderedSequence(encryptionContext.Keys, UInt.UInt8Less);
+      var kvPairs := seq(|keys|, i requires 0 <= i < |keys| => (keys[i], encryptionContext[keys[i]]));
+      2 + KVPairEntriesLength(kvPairs, 0, |kvPairs|)
+  }
+
+  /*
+   * Encryption context as a sequence
+   */
+
+  // To make verification and working with iterating through the encryption context
+  // simpler, here we define a specific type to represent a sequence of key-value tuples.
+  type Linear = seq<(UTF8.ValidUTF8Bytes, UTF8.ValidUTF8Bytes)>
+
+  // Length of KVPairEntries is defined in terms of a seq of tuples, which is easier to reason about
+  function KVPairEntriesLength(kvPairs: Linear, lo: nat, hi: nat): nat
+    requires lo <= hi <= |kvPairs|
+  {
+    if lo == hi then 0 else
+      KVPairEntriesLength(kvPairs, lo, hi - 1) +
+      2 + |kvPairs[hi - 1].0| +
+      2 + |kvPairs[hi - 1].1|
+  }
+
+  // There isn't an efficient way to build a map from a sequence in dafny, so this
+  // extern is used specifically to convert a sequence of key value pairs to a map
+  method {:extern "KVPairSequenceToMap"} KVPairSequenceToMap(kvPairs: Linear) returns (res: T)  // TODO: FromLinear
+
+  /*
+   * Useful lemmas about key-value pairs
+   */
+
+  lemma KVPairEntriesLengthSplit(kvPairs: Linear, lo: nat, mid: nat, hi: nat)
+    requires lo <= mid <= hi <= |kvPairs|
+    ensures KVPairEntriesLength(kvPairs, lo, hi)
+         == KVPairEntriesLength(kvPairs, lo, mid) + KVPairEntriesLength(kvPairs, mid, hi)
+  {
+  }
+
+  lemma KVPairEntriesLengthPrefix(kvPairs: Linear, more: Linear)
+    ensures KVPairEntriesLength(kvPairs + more, 0, |kvPairs|) == KVPairEntriesLength(kvPairs, 0, |kvPairs|)
+  {
+    var n := |kvPairs|;
+    if n == 0 {
+    } else {
+      var last := kvPairs[n - 1];
+      calc {
+        KVPairEntriesLength(kvPairs + more, 0, n);
+      ==  // def. KVPairEntriesLength
+        KVPairEntriesLength(kvPairs + more, 0, n - 1) + 4 + |last.0| + |last.1|;
+      ==  { assert kvPairs + more == kvPairs[..n - 1] + ([last] + more); }
+        KVPairEntriesLength(kvPairs[..n - 1] + ([last] + more), 0, n - 1) + 4 + |last.0| + |last.1|;
+      ==  { KVPairEntriesLengthPrefix(kvPairs[..n - 1], [last] + more); }
+        KVPairEntriesLength(kvPairs[..n - 1], 0, n - 1) + 4 + |last.0| + |last.1|;
+      ==  { KVPairEntriesLengthPrefix(kvPairs[..n - 1], [last] + more); }
+        KVPairEntriesLength(kvPairs[..n - 1] + [last], 0, n - 1) + 4 + |last.0| + |last.1|;
+      ==  { assert kvPairs[..n - 1] + [last] == kvPairs; }
+        KVPairEntriesLength(kvPairs, 0, n - 1) + 4 + |last.0| + |last.1|;
+      ==  // def. KVPairEntriesLength
+        KVPairEntriesLength(kvPairs, 0, n);
+      }
+    }
+  }
+
+  lemma KVPairEntriesLengthExtend(kvPairs: Linear, key: UTF8.ValidUTF8Bytes, value: UTF8.ValidUTF8Bytes)
+    ensures KVPairEntriesLength(kvPairs + [(key, value)], 0, |kvPairs| + 1)
+         == KVPairEntriesLength(kvPairs, 0, |kvPairs|) + 4 + |key| + |value|
+  {
+    KVPairEntriesLengthPrefix(kvPairs, [(key, value)]);
+  }
+
+  lemma KVPairEntriesLengthInsert(kvPairs: Linear, insertionPoint: nat, key: UTF8.ValidUTF8Bytes, value: UTF8.ValidUTF8Bytes)
+    requires insertionPoint <= |kvPairs|
+    ensures var kvPairs' := kvPairs[..insertionPoint] + [(key, value)] + kvPairs[insertionPoint..];
+      KVPairEntriesLength(kvPairs', 0, |kvPairs'|) == KVPairEntriesLength(kvPairs, 0, |kvPairs|) + 4 + |key| + |value|
+    decreases |kvPairs|
+  {
+    var kvPairs' := kvPairs[..insertionPoint] + [(key, value)] + kvPairs[insertionPoint..];
+    if |kvPairs| == insertionPoint {
+      assert kvPairs' == kvPairs + [(key, value)];
+      KVPairEntriesLengthExtend(kvPairs, key, value);
+    } else {
+      var m := |kvPairs| - 1;
+      var (d0, d1) := kvPairs[m];
+      var a, b, c, d := kvPairs[..insertionPoint], [(key, value)], kvPairs[insertionPoint..m], [(d0, d1)];
+      assert kvPairs == a + c + d;
+      assert kvPairs' == a + b + c + d;
+      var ac := a + c;
+      var abc := a + b + c;
+      calc {
+        KVPairEntriesLength(kvPairs', 0, |kvPairs'|);
+        KVPairEntriesLength(abc + [(d0, d1)], 0, |abc| + 1);
+      ==  { KVPairEntriesLengthExtend(abc, d0, d1); }
+        KVPairEntriesLength(abc, 0, |abc|) + 4 + |d0| + |d1|;
+      ==  { KVPairEntriesLengthInsert(ac, insertionPoint, key, value); }
+        KVPairEntriesLength(ac, 0, |ac|) + 4 + |key| + |value| + 4 + |d0| + |d1|;
+      ==  { KVPairEntriesLengthExtend(ac, d0, d1); }
+        KVPairEntriesLength(kvPairs, 0, |kvPairs|) + 4 + |key| + |value|;
+      }
+    }
+  }
+
+  /*
+   * Methods that compute properties of encryption contexts
+   */
+
+  method ComputeKVPairsLength(encryptionContext: T) returns (res: nat)
+    ensures res as nat == KVPairsLength(encryptionContext)
+  {
+    reveal ValidAAD();
+    if |encryptionContext| == 0 {
+      return 0;
+    }
+
+    // Iterating through a map isn't feasbile in dafny for large maps, so instead
+    // convert the map to a sequence of key pairs and iterate through the sequence
+    var keys: seq<UTF8.ValidUTF8Bytes> := Sets.ComputeSetToOrderedSequence(encryptionContext.Keys, UInt.UInt8Less);
+    var kvPairs := seq(|keys|, i requires 0 <= i < |keys| => (keys[i], encryptionContext[keys[i]]));
+
+    var len := 2;
+    var i := 0;
+    while i < |kvPairs|
+      invariant i <= |kvPairs|
+      invariant 2 + KVPairEntriesLength(kvPairs, 0, i as int) == len as int
+    {
+      var kvPair := kvPairs[i];
+      len := len + 4 + |kvPair.0| + |kvPair.1|;
+      KVPairEntriesLengthSplit(kvPairs, 0, i + 1, |kvPairs| as int);
+      i := i + 1;
+    }
+
+    assert len == 2 + KVPairEntriesLength(kvPairs, 0, |kvPairs|);
+    assert len == KVPairsLength(encryptionContext);
+
+    return len;
+  }
+
+  method ComputeValidAAD(encryptionContext: T) returns (res: bool)
+    ensures res == ValidAAD(encryptionContext)
+  {
+    reveal ValidAAD();
+
+    if |encryptionContext| == 0 {
+      return true;
+    } else if |encryptionContext| >= UINT16_LIMIT {
+      return false;
+    }
+    
+    // Iterating through a map isn't feasbile in dafny for large maps, so instead
+    // convert the map to a sequence of key pairs and iterate through the sequence
+    var keys: seq<UTF8.ValidUTF8Bytes> := Sets.ComputeSetToOrderedSequence<uint8>(encryptionContext.Keys, UInt.UInt8Less);
+    var kvPairs := seq(|keys|, i requires 0 <= i < |keys| => (keys[i], encryptionContext[keys[i]]));
+    assert forall i :: 0 <= i < |keys| ==> kvPairs[i] == (keys[i], encryptionContext[keys[i]]);
+
+    var kvPairsLen := 2;
+    var i := 0;
+    while i < |kvPairs|
+      invariant i <= |kvPairs|
+      invariant forall k :: 0 <= k < i ==> ValidKVPair(kvPairs[k])
+      invariant 2 + KVPairEntriesLength(kvPairs, 0, i as int) == kvPairsLen as int < UINT16_LIMIT
+    {
+      var kvPair := kvPairs[i];
+      kvPairsLen := kvPairsLen + 4 + |kvPair.0| + |kvPair.1|;
+      KVPairEntriesLengthSplit(kvPairs, 0, i as int + 1, |kvPairs| as int);
+
+      // Check that AAD is still valid with this pair
+      if !(|kvPair.0| < UINT16_LIMIT && |kvPair.1| < UINT16_LIMIT) {
+        assert kvPair.0 in encryptionContext.Keys;
+        return false; // Invalid key value pair
+      } else if kvPairsLen >= UINT16_LIMIT {
+        return false; // Over size limit
+      }
+      assert forall k :: 0 <= k < i ==> ValidKVPair(kvPairs[k]);
+      assert kvPairsLen < UINT16_LIMIT;
+      i := i + 1;
+    }
+
+    return true;
+  }
+
+  /*
+   * Sortedness
+   */
+
+  predicate SortedKVPairsUpTo(a: Linear, n: nat)
+    requires n <= |a|
+  {
+    forall j :: 0 < j < n ==> LexicographicLessOrEqual(a[j-1].0, a[j].0, UInt.UInt8Less)
+  }
+
+  predicate SortedKVPairs(kvPairs: Linear)
+  {
+    SortedKVPairsUpTo(kvPairs, |kvPairs|)
+  }
+
+  function AADToSeq(kvPairs: T): seq<uint8>
+    requires ValidAAD(kvPairs)
+  {
+    reveal ValidAAD();
+    UInt16ToSeq(KVPairsLength(kvPairs) as uint16) +
+    KVPairsToSeq(kvPairs)
+  }
+
+  function KVPairsToSeq(kvPairs: T): seq<uint8>
+    requires ValidKVPairs(kvPairs)
+  {
+    var n := |kvPairs|;
+    if n == 0 then [] else
+      // Defining and reasoning about order at this level is simplified by using a sequence of
+      // key value pairs instead of a map.
+      // Pairs are ordered lexicographically by their UTF8 encoding, which is equivalent to code
+      // point ordering.
+      var keys: seq<UTF8.ValidUTF8Bytes> := SetToOrderedSequence<uint8>(kvPairs.Keys, UInt.UInt8Less);
+      var kvPairsSeq := seq(|keys|, i requires 0 <= i < |keys| => (keys[i], kvPairs[keys[i]]));
+      UInt16ToSeq(n as uint16) +
+      KVPairEntriesToSeq(kvPairsSeq, 0, |kvPairsSeq|)
+  }
+
+  // Serialization of KVPairEntries is defined in terms of a seq of tuples, which is easier to reason about
+  function KVPairEntriesToSeq(kvPairs: Linear, lo: nat, hi: nat): seq<uint8>
+    requires forall i :: 0 <= i < |kvPairs| ==> ValidKVPair(kvPairs[i])
+    requires |kvPairs| < UINT16_LIMIT
+    requires SortedKVPairs(kvPairs)
+    requires lo <= hi <= |kvPairs|
+  {
+    if lo == hi then [] else KVPairEntriesToSeq(kvPairs, lo, hi - 1) + KVPairToSeq(kvPairs[hi - 1])
+  }
+
+  function KVPairToSeq(kvPair: (UTF8.ValidUTF8Bytes, UTF8.ValidUTF8Bytes)): seq<uint8>
+    requires ValidKVPair(kvPair)
+  {
+    UInt16ToSeq(|kvPair.0| as uint16) + kvPair.0 +
+    UInt16ToSeq(|kvPair.1| as uint16) + kvPair.1
+  }
+
+  /* Function KVPairsLength is defined without referring to SerializeAAD (because then
+   * these two would be mutually recursive with ValidAAD). The following lemma proves
+   * that the two definitions correspond.
+   */
+
+  lemma ADDLengthCorrect(encryptionContext: T)
+    requires ValidAAD(encryptionContext)
+    ensures |AADToSeq(encryptionContext)| == 2 + KVPairsLength(encryptionContext)
+  {
+    reveal ValidAAD();
+    var keys: seq<UTF8.ValidUTF8Bytes> := SetToOrderedSequence(encryptionContext.Keys, UInt.UInt8Less);
+    var kvPairs := seq(|keys|, i requires 0 <= i < |keys| => (keys[i], encryptionContext[keys[i]]));
+    KVPairEntriesLengthCorrect(kvPairs, 0, |kvPairs|);
+    /**** Here's a more detailed proof:
+    var n := |kvPairs|;
+    if n != 0 {
+      var s := KVPairEntriesToSeq(kvPairs, 0, n);
+      calc {
+        |AADToSeq(kvPairs)|;
+      ==  // def. AADToSeq
+        |UInt16ToSeq(KVPairsLength(kvPairs) as uint16) + UInt16ToSeq(n as uint16) + s|;
+      ==  // UInt16ToSeq yields length-2 sequence
+        2 + 2 + |s|;
+      ==  { KVPairEntriesLengthCorrect(kvPairs, 0, n); }
+        2 + 2 + KVPairEntriesLength(kvPairs, 0, n);
+      }
+    }
+    ****/
+  }
+
+  lemma KVPairEntriesLengthCorrect(encryptionContext: Linear, lo: nat, hi: nat)
+    requires forall i :: 0 <= i < |encryptionContext| ==> ValidKVPair(encryptionContext[i])
+    requires lo <= hi <= |encryptionContext|
+    requires |encryptionContext| < UINT16_LIMIT
+    requires SortedKVPairs(encryptionContext)
+    ensures |KVPairEntriesToSeq(encryptionContext, lo, hi)| == KVPairEntriesLength(encryptionContext, lo, hi)
+  {
+    /**** Here's a more detailed proof:
+    if lo < hi {
+      var kvPair := kvPairs[hi - 1];
+      calc {
+        |KVPairEntriesToSeq(kvPairs, lo, hi)|;
+      ==  // def. KVPairEntriesToSeq
+        |KVPairEntriesToSeq(kvPairs, lo, hi - 1) + KVPairToSeq(kvPair)|;
+      ==
+        |KVPairEntriesToSeq(kvPairs, lo, hi - 1)| + |KVPairToSeq(kvPair)|;
+      ==  { KVPairEntriesLengthCorrect(kvPairs, lo, hi - 1); }
+        KVPairEntriesLength(kvPairs, lo, hi - 1) + |KVPairToSeq(kvPair)|;
+      ==  // def. KVPairToSeq
+        KVPairEntriesLength(kvPairs, lo, hi - 1) +
+        |UInt16ToSeq(|kvPair.0| as uint16) + kvPair.0 + UInt16ToSeq(|kvPair.1| as uint16) + kvPair.1|;
+      ==
+        KVPairEntriesLength(kvPairs, lo, hi - 1) + 2 + |kvPair.0| + 2 + |kvPair.1|;
+      ==  // def. KVPairEntriesLength
+        KVPairEntriesLength(kvPairs, lo, hi);
+      }
+    }
+    ****/
+  }
+}
